rename with snake_case

Projects/Lindmar_Joost/BinaryHeapTreeV.lean
@@ -10,16 +10,16 @@ inductive BinaryTree (α : Type u)
 
 namespace BinaryTree
 
-@[grind] def isMinHeap : BinaryTree α → (dist : α → ENat) → Prop
+@[grind] def is_min_heap : BinaryTree α → (dist : α → ENat) → Prop
 | leaf, _ => true
 | node l v r, f => match l, r with
       | leaf, leaf => true
       | node _ lv _, leaf =>
-          f v <= f lv ∧ isMinHeap l f
+          f v <= f lv ∧ is_min_heap l f
       | leaf, node _ rv _ =>
-          f v <= f rv ∧ isMinHeap r f
+          f v <= f rv ∧ is_min_heap r f
       | node _ lv _, node _ rv _ =>
-          f v <= f lv ∧ isMinHeap l f ∧ f v <= f rv ∧ isMinHeap r f
+          f v <= f lv ∧ is_min_heap l f ∧ f v <= f rv ∧ is_min_heap r f
 
 @[grind] def heapify (bt: BinaryTree α) (f: α → ENat): BinaryTree α := match bt with
 | leaf => bt
@@ -34,24 +34,24 @@ namespace BinaryTree
                                           if f v <= f rv then bt
                                           else node l rv (heapify (node rl v rr) f)
 
-@[grind] def getLast: BinaryTree α → Option α ×  BinaryTree α
+@[grind] def get_last: BinaryTree α → Option α ×  BinaryTree α
 | leaf => (none, leaf)
 | node l v r => match l, r with
     | leaf, leaf => (some v, leaf)
-    | leaf, _ => let (val, tree) := (getLast r)
+    | leaf, _ => let (val, tree) := (get_last r)
       (val, node l v tree)
-    | _, _ => let (val, tree) := (getLast l)
+    | _, _ => let (val, tree) := (get_last l)
       (val, node tree v r)
 
-@[grind] def extractMin (bt: BinaryTree α) (f: α → ENat): (Option α × BinaryTree α):=
-let (lastNode, treeWithoutLast) := getLast bt
+@[grind] def extract_min (bt: BinaryTree α) (f: α → ENat): (Option α × BinaryTree α):=
+let (lastNode, treeWithoutLast) := get_last bt
 match lastNode with
 | none => (none, leaf)
 | some v' => match treeWithoutLast with
   | leaf => (some v', leaf)
   | node l v r => (some v, heapify (node l v' r) f)
 
-@[grind] def heapMin:  BinaryTree α → (α → ENat) → ENat
+@[grind] def heap_min:  BinaryTree α → (α → ENat) → ENat
 | leaf, _ => ⊤
 | node l v r, f => match l, r with
     | leaf, leaf => (f v)
@@ -65,7 +65,7 @@ match lastNode with
                                       else f rv
 
 
-@[grind] def rootIsMinOfChildren: (BinaryTree α) → (α → ENat) →  Prop
+@[grind] def root_is_min_of_children: (BinaryTree α) → (α → ENat) →  Prop
 | leaf, _ => true
 | node l v r, f => match l, r with
     | leaf, leaf => true
@@ -74,18 +74,18 @@ match lastNode with
     | node _ lv _, node _ rv _ =>  f v <= f lv ∧ f v <= f rv
 
 
-@[grind] def leftAndRightAreMinHeap: (BinaryTree α) →  (f: α → ENat) →  Prop
+@[grind] def left_and_right_are_min_heap: (BinaryTree α) →  (f: α → ENat) →  Prop
 | leaf, _ => true
-| node l _ r, f => isMinHeap l f ∧ isMinHeap r f
+| node l _ r, f => is_min_heap l f ∧ is_min_heap r f
 
 @[grind] def contains : (BinaryTree α) → α → Prop
 | leaf, _ => false
 | node l v r, v' => v = v' ∨ contains l v' ∨ contains r v'
 
 
-@[grind] def containsB [DecidableEq α] : (BinaryTree α) → α → Bool
+@[grind] def containsb [DecidableEq α] : (BinaryTree α) → α → Bool
 | leaf, _ => false
-| node l v r, v' => (v = v') ∨ containsB l v' ∨ containsB r v'
+| node l v r, v' => (v = v') ∨ containsb l v' ∨ containsb r v'
 
 @[grind] def insert (bt : BinaryTree α) (v : α) (f : α → ENat) : BinaryTree α :=
   match bt with
@@ -97,27 +97,27 @@ match lastNode with
       else
         node (insert l v f) x r
 
-lemma minHeapThenLeftAndRightAreMinHeap (bt: BinaryTree α) (f: α → ENat): isMinHeap bt f → leftAndRightAreMinHeap bt f := by
+lemma min_heap_then_left_and_right_are_min_heap (bt: BinaryTree α) (f: α → ENat): is_min_heap bt f → left_and_right_are_min_heap bt f := by
 intro hbt
-fun_induction isMinHeap; all_goals (grind [leftAndRightAreMinHeap, isMinHeap])
+fun_induction is_min_heap; all_goals (grind [left_and_right_are_min_heap, is_min_heap])
 
-lemma minHeapThenRootIsMinOfChildren (bt: BinaryTree α) (f: α → ENat): isMinHeap bt f → rootIsMinOfChildren bt f := by
+lemma min_heap_then_root_is_min_of_children (bt: BinaryTree α) (f: α → ENat): is_min_heap bt f → root_is_min_of_children bt f := by
 intro hbt
-fun_induction isMinHeap; all_goals (grind [rootIsMinOfChildren])
+fun_induction is_min_heap; all_goals (grind [root_is_min_of_children])
 
-lemma leftAndRightAreMinHeapAndRootIsMinOfChildrenToMinHeap (bt: BinaryTree α) (f: α → ENat): leftAndRightAreMinHeap bt f ∧ rootIsMinOfChildren bt f → isMinHeap bt f := by
+lemma left_and_right_are_min_heap_and_root_is_min_of_children_is_min_heap (bt: BinaryTree α) (f: α → ENat): left_and_right_are_min_heap bt f ∧ root_is_min_of_children bt f → is_min_heap bt f := by
 intro hbt
-fun_induction isMinHeap; all_goals (simp [rootIsMinOfChildren, leftAndRightAreMinHeap] at hbt;simp[hbt])
+fun_induction is_min_heap; all_goals (simp [root_is_min_of_children, left_and_right_are_min_heap] at hbt;simp[hbt])
 
-lemma leftAndRightAreMinHeapLeft (l: BinaryTree α) (r: BinaryTree α) (v: α) (f: α → ENat): leftAndRightAreMinHeap (node l v r) f → leftAndRightAreMinHeap l f := by
+lemma left_and_right_are_min_heapLeft (l: BinaryTree α) (r: BinaryTree α) (v: α) (f: α → ENat): left_and_right_are_min_heap (node l v r) f → left_and_right_are_min_heap l f := by
 intro hbt
-simp [leftAndRightAreMinHeap] at hbt
-simp [minHeapThenLeftAndRightAreMinHeap, hbt]
+simp [left_and_right_are_min_heap] at hbt
+simp [min_heap_then_left_and_right_are_min_heap, hbt]
 
-lemma leftAndRightAreMinHeapRight (l: BinaryTree α) (r: BinaryTree α) (v: α) (f: α → ENat): leftAndRightAreMinHeap (node l v r) f → leftAndRightAreMinHeap r f := by
+lemma left_and_right_are_min_heapRight (l: BinaryTree α) (r: BinaryTree α) (v: α) (f: α → ENat): left_and_right_are_min_heap (node l v r) f → left_and_right_are_min_heap r f := by
 intro hbt
-simp [leftAndRightAreMinHeap] at hbt
-simp [minHeapThenLeftAndRightAreMinHeap, hbt]
+simp [left_and_right_are_min_heap] at hbt
+simp [min_heap_then_left_and_right_are_min_heap, hbt]
 
 lemma heapifyPreservesStructure (bt: BinaryTree α) (f: α → ENat): (∃ l r v, bt = node l v r) →  ∃ l' v' r', heapify bt f = node l' v' r' := by
 intro hbt
@@ -126,40 +126,38 @@ fun_induction heapify; all_goals expose_names
   contradiction
 all_goals simp
 
-lemma heapifyPreservesStructureAndRootMin (bt: BinaryTree α) (f: α → ENat): (∃ l r v, bt = node l v r) →  ∃ l' v' r', heapify bt f = node l' v' r' ∧ f v' ≤ (heapMin bt f) := by
+lemma heapify_preserves_structure_and_root_min (bt: BinaryTree α) (f: α → ENat): (∃ l r v, bt = node l v r) →  ∃ l' v' r', heapify bt f = node l' v' r' ∧ f v' ≤ (heap_min bt f) := by
 intro hbt
 fun_induction heapify; all_goals expose_names
 . obtain ⟨l, r, v, hbt⟩ := hbt
   contradiction
-all_goals grind [heapMin]
+all_goals grind [heap_min]
 
-lemma heapifyPreservesMembers (bt: BinaryTree α) (v: α) (f: α → ENat): contains bt v → contains (heapify bt f) v := by
-intro hbt
+lemma contains_then_heapify_contains (bt: BinaryTree α) (v: α) (f: α → ENat): contains bt v → contains (heapify bt f) v := by
 fun_induction heapify generalizing v; all_goals try grind[contains]
 
-lemma heapifyPreservesMembers2 (bt: BinaryTree α) (v: α) (f: α → ENat):  contains (heapify bt f) v → contains bt v := by
-intro hbt
+lemma heapify_contains_then_contains (bt: BinaryTree α) (v: α) (f: α → ENat):  contains (heapify bt f) v → contains bt v := by
 fun_induction heapify generalizing v; all_goals try grind[contains]
 
-lemma containsIsNode (bt: BinaryTree α) (v: α): contains bt v → ∃ l v' r, bt = node l v' r := by
+lemma contains_is_node (bt: BinaryTree α) (v: α): contains bt v → ∃ l v' r, bt = node l v' r := by
 fun_induction contains; all_goals simp
 
-lemma minHeapRootMin (bt l r: BinaryTree α) (v: α) (f: α → ENat): bt = (node l v r) → isMinHeap bt f → f v = heapMin bt f := by
+lemma min_heap_root_min (bt l r: BinaryTree α) (v: α) (f: α → ENat): bt = (node l v r) → is_min_heap bt f → f v = heap_min bt f := by
 intro hbt hmin
-fun_induction isMinHeap; all_goals grind [heapMin]
+fun_induction is_min_heap; all_goals grind [heap_min]
 
-lemma rootIsMinOfChildrenLeft (l r ll lr: BinaryTree α) (v lv: α) (f: α → ENat): rootIsMinOfChildren (node l v r) f →  l = (node ll lv lr) →  f v ≤ f lv := by
+lemma root_is_min_of_children_left (l r ll lr: BinaryTree α) (v lv: α) (f: α → ENat): root_is_min_of_children (node l v r) f →  l = (node ll lv lr) →  f v ≤ f lv := by
   intros; expose_names
   rw [h_1] at h
-  cases r; all_goals grind[rootIsMinOfChildren]
+  cases r; all_goals grind[root_is_min_of_children]
 
-lemma rootIsMinOfChildrenRight (l r rl rr: BinaryTree α) (v rv: α) (f: α → ENat): rootIsMinOfChildren (node l v r) f →  r = (node rl rv rr) → f v ≤ f rv := by
+lemma root_is_min_of_children_right (l r rl rr: BinaryTree α) (v rv: α) (f: α → ENat): root_is_min_of_children (node l v r) f →  r = (node rl rv rr) → f v ≤ f rv := by
   intros; expose_names
   rw [h_1] at h
-  cases r; all_goals try grind[rootIsMinOfChildren]
-  . grind [rootIsMinOfChildren.eq_def]
+  cases r; all_goals try grind[root_is_min_of_children]
+  . grind [root_is_min_of_children.eq_def]
 
-lemma minHeapMemberLeRoot (bt: BinaryTree α) (v: α) (f: α → ENat): isMinHeap bt f →  contains bt v →  heapMin bt f ≤ f v := by
+lemma min_heap_member_le_root (bt: BinaryTree α) (v: α) (f: α → ENat): is_min_heap bt f →  contains bt v →  heap_min bt f ≤ f v := by
 intro hmin hl
 fun_induction contains
 . contradiction
@@ -167,49 +165,49 @@ fun_induction contains
   cases hl; all_goals expose_names
   . expose_names
     rw [←h]
-    suffices f v = (l.node v r).heapMin f by grind
-    apply minHeapRootMin (l.node v r) l r v; all_goals grind
+    suffices f v = (l.node v r).heap_min f by grind
+    apply min_heap_root_min (l.node v r) l r v; all_goals grind
   . cases h; all_goals expose_names
     . have h2: l.contains v' := by exact h
-      apply containsIsNode at h2
+      apply contains_is_node at h2
       obtain ⟨l'', v'', r'', h2 ⟩:= h2
       have h3: l = l''.node v'' r'' := by exact h2
-      have hmin2: (l.node v r).isMinHeap f := by assumption
-      have hmin3: (l.node v r).isMinHeap f := by assumption
-      apply minHeapThenLeftAndRightAreMinHeap at hmin
-      simp [leftAndRightAreMinHeap] at hmin
-      have hlmin: l.isMinHeap f:= by grind
-      have hlmin2: l.isMinHeap f:= by grind
+      have hmin2: (l.node v r).is_min_heap f := by assumption
+      have hmin3: (l.node v r).is_min_heap f := by assumption
+      apply min_heap_then_left_and_right_are_min_heap at hmin
+      simp [left_and_right_are_min_heap] at hmin
+      have hlmin: l.is_min_heap f:= by grind
+      have hlmin2: l.is_min_heap f:= by grind
       apply ih2 at hlmin
       apply hlmin at h
       grw[← h]
-      apply minHeapThenRootIsMinOfChildren at hmin2
-      apply rootIsMinOfChildrenLeft l r l'' r'' v v'' f hmin2 at h2
-      have hhl: f v'' = l.heapMin f:= by grind [minHeapRootMin]
-      have hh: f v = (l.node v r).heapMin f:= by grind [minHeapRootMin]
+      apply min_heap_then_root_is_min_of_children at hmin2
+      apply root_is_min_of_children_left l r l'' r'' v v'' f hmin2 at h2
+      have hhl: f v'' = l.heap_min f:= by grind [min_heap_root_min]
+      have hh: f v = (l.node v r).heap_min f:= by grind [min_heap_root_min]
       grw [← hh, ← hhl]
       exact h2
     . have h2: r.contains v' := by exact h
-      apply containsIsNode at h2
+      apply contains_is_node at h2
       obtain ⟨l'', v'', r'', h2 ⟩:= h2
       have h3: r = l''.node v'' r'' := by exact h2
-      have hmin2: (l.node v r).isMinHeap f:= by assumption
-      have hmin3: (l.node v r).isMinHeap f:= by assumption
-      apply minHeapThenLeftAndRightAreMinHeap at hmin
-      simp [leftAndRightAreMinHeap] at hmin
-      have hlmin: r.isMinHeap f:= by grind
-      have hlmin2: r.isMinHeap f:= by grind
+      have hmin2: (l.node v r).is_min_heap f:= by assumption
+      have hmin3: (l.node v r).is_min_heap f:= by assumption
+      apply min_heap_then_left_and_right_are_min_heap at hmin
+      simp [left_and_right_are_min_heap] at hmin
+      have hlmin: r.is_min_heap f:= by grind
+      have hlmin2: r.is_min_heap f:= by grind
       apply ih1 at hlmin
       apply hlmin at h
       grw[← h]
-      apply minHeapThenRootIsMinOfChildren at hmin2
-      apply rootIsMinOfChildrenRight l r l'' r'' v v'' f hmin2 at h2
-      have hhl: f v'' = r.heapMin f:= by grind [minHeapRootMin]
-      have hh: f v = (l.node v r).heapMin f:= by grind [minHeapRootMin]
+      apply min_heap_then_root_is_min_of_children at hmin2
+      apply root_is_min_of_children_right l r l'' r'' v v'' f hmin2 at h2
+      have hhl: f v'' = r.heap_min f:= by grind [min_heap_root_min]
+      have hh: f v = (l.node v r).heap_min f:= by grind [min_heap_root_min]
       grw [← hh, ← hhl]
       exact h2
 
-lemma minHeapContainsLeRoot (bt l r: BinaryTree α) (v v': α) (f: α → ENat): isMinHeap bt f → bt = node l v r → contains bt v' → f v ≤ f v' := by
+lemma min_heap_contains_le_root (bt l r: BinaryTree α) (v v': α) (f: α → ENat): is_min_heap bt f → bt = node l v r → contains bt v' → f v ≤ f v' := by
 intro hmin hbt hv'
 fun_induction contains generalizing l v r
 . contradiction
@@ -217,96 +215,96 @@ fun_induction contains generalizing l v r
   cases hv'; all_goals expose_names
   . simp_all
   . cases h; all_goals expose_names
-    . obtain ⟨ ll, lv, lr, hl ⟩ := containsIsNode l_1 v' h
+    . obtain ⟨ ll, lv, lr, hl ⟩ := contains_is_node l_1 v' h
       have: f lv ≤ f v' := by
         apply ih2 ll lr lv _ hl h
-        apply minHeapThenLeftAndRightAreMinHeap at hmin
-        rw [leftAndRightAreMinHeap] at hmin
+        apply min_heap_then_left_and_right_are_min_heap at hmin
+        rw [left_and_right_are_min_heap] at hmin
         obtain ⟨ hl', hr' ⟩ := hmin
         exact hl'
       grw [←this]
-      apply rootIsMinOfChildrenLeft l r ll lr v lv f (by grind [minHeapThenRootIsMinOfChildren]) (by grind)
-    . obtain ⟨ rl, rv, rr, hr ⟩ := containsIsNode r_1 v' h
+      apply root_is_min_of_children_left l r ll lr v lv f (by grind [min_heap_then_root_is_min_of_children]) (by grind)
+    . obtain ⟨ rl, rv, rr, hr ⟩ := contains_is_node r_1 v' h
       have: f rv ≤ f v' := by
         apply ih1 rl rr rv _ hr h
-        apply minHeapThenLeftAndRightAreMinHeap at hmin
-        rw [leftAndRightAreMinHeap] at hmin
+        apply min_heap_then_left_and_right_are_min_heap at hmin
+        rw [left_and_right_are_min_heap] at hmin
         obtain ⟨ hl', hr' ⟩ := hmin
         exact hr'
       grw [←this]
-      apply rootIsMinOfChildrenRight l r rl rr v rv f (by grind [minHeapThenRootIsMinOfChildren]) (by grind)
+      apply root_is_min_of_children_right l r rl rr v rv f (by grind [min_heap_then_root_is_min_of_children]) (by grind)
 
-lemma heapifyPreservesMinHeap (bt: BinaryTree α) (f: α → ENat): isMinHeap bt f → bt = heapify bt f:= by
+lemma heapify_preserves_min_heap (bt: BinaryTree α) (f: α → ENat): is_min_heap bt f → bt = heapify bt f:= by
 fun_induction heapify; all_goals expose_names; all_goals try grind
 
-lemma binTreeEqR (l r l' r': BinaryTree α) (v v': α): (node l v r) = (node l' v' r') → r = r' := by
+lemma binary_tree_eq_r (l r l' r': BinaryTree α) (v v': α): (node l v r) = (node l' v' r') → r = r' := by
 grind only
 
-lemma binTreeEqL (l r l' r': BinaryTree α) (v v': α): (node l v r) = (node l' v' r') → l = l' := by
+lemma binary_tree_eq_l (l r l' r': BinaryTree α) (v v': α): (node l v r) = (node l' v' r') → l = l' := by
 grind only
 
-lemma heapifyPreservesValues (tree r l: BinaryTree α) (v: α) (f: α → ENat): tree.heapify f = node r v l → contains tree v := by
-grind [contains, heapifyPreservesMembers2]
+lemma heapify_preserves_values (tree r l: BinaryTree α) (v: α) (f: α → ENat): tree.heapify f = node r v l → contains tree v := by
+grind [contains, heapify_contains_then_contains]
 
-lemma containsRootOrChildren (tree r l: BinaryTree α) (v v': α) : tree = node r v l → contains tree v' → contains r v' ∨ contains l v' ∨ v= v' := by
+lemma contains_root_or_children (tree r l: BinaryTree α) (v v': α) : tree = node r v l → contains tree v' → contains r v' ∨ contains l v' ∨ v= v' := by
 grind [contains]
 
-lemma containsRootOrChildrenLeftLeaf (tree r: BinaryTree α) (v v':  α): tree = node r v leaf → contains tree v' → contains r v' ∨ v= v' := by
+lemma contains_root_or_children_left_leaf (tree r: BinaryTree α) (v v':  α): tree = node r v leaf → contains tree v' → contains r v' ∨ v= v' := by
 grind [contains]
 
-lemma containsRightThenContainsRoot (tree l r: BinaryTree α) (v v':  α): tree = node l v r → contains r v' → contains tree v' := by
+lemma contains_right_then_contains_root (tree l r: BinaryTree α) (v v':  α): tree = node l v r → contains r v' → contains tree v' := by
 grind [contains]
 
-lemma containsLeftThenContainsRoot (tree l r: BinaryTree α) (v v':  α): tree = node l v r → contains l v' → contains tree v' := by
+lemma contains_left_then_contains_root (tree l r: BinaryTree α) (v v':  α): tree = node l v r → contains l v' → contains tree v' := by
 grind [contains]
 
-lemma minHeapThenMembersLeftLe (bt l r: BinaryTree α) (v v': α) (f: α → ENat): isMinHeap bt f → bt = node l v r → contains l v' → f v ≤ f v' := by
+lemma min_heap_then_members_left_le (bt l r: BinaryTree α) (v v': α) (f: α → ENat): is_min_heap bt f → bt = node l v r → contains l v' → f v ≤ f v' := by
 intro hmin hbt hl
-apply containsLeftThenContainsRoot bt l r v v' hbt at hl
-apply minHeapContainsLeRoot bt l r v v' f hmin hbt hl
+apply contains_left_then_contains_root bt l r v v' hbt at hl
+apply min_heap_contains_le_root bt l r v v' f hmin hbt hl
 
-lemma minHeapThenMembersRightLe (bt l r: BinaryTree α) (v v': α) (f: α → ENat): isMinHeap bt f → bt = node l v r → contains r v' → f v ≤ f v' := by
+lemma min_heap_then_members_right_le (bt l r: BinaryTree α) (v v': α) (f: α → ENat): is_min_heap bt f → bt = node l v r → contains r v' → f v ≤ f v' := by
 intro hmin hbt hl
-apply containsRightThenContainsRoot bt l r v v' hbt at hl
-apply minHeapContainsLeRoot bt l r v v' f hmin hbt hl
+apply contains_right_then_contains_root bt l r v v' hbt at hl
+apply min_heap_contains_le_root bt l r v v' f hmin hbt hl
 
-lemma heapifyEstablishesMinHeap' {α} (bt l r: BinaryTree α) (v: α) (f: α → ENat): bt = node l v r ∧  isMinHeap l f ∧ isMinHeap r f → isMinHeap (heapify bt f) f := by
+lemma heapify_establishes_min_heap {α} (bt l r: BinaryTree α) (v: α) (f: α → ENat): bt = node l v r ∧  is_min_heap l f ∧ is_min_heap r f → is_min_heap (heapify bt f) f := by
 fun_induction heapify generalizing l r v; all_goals expose_names
-. simp [isMinHeap]
-. simp [isMinHeap]
+. simp [is_min_heap]
+. simp [is_min_heap]
 . intro ⟨hr, hminl, hminr⟩
-  apply leftAndRightAreMinHeapAndRootIsMinOfChildrenToMinHeap
-  have: ∃ rl' v' rr', (rl.node v_1 rr).heapify f = node rl' v' rr' ∧ f v' ≤ heapMin (rl.node v_1 rr) f:= by
-        apply heapifyPreservesStructureAndRootMin
+  apply left_and_right_are_min_heap_and_root_is_min_of_children_is_min_heap
+  have: ∃ rl' v' rr', (rl.node v_1 rr).heapify f = node rl' v' rr' ∧ f v' ≤ heap_min (rl.node v_1 rr) f:= by
+        apply heapify_preserves_structure_and_root_min
         simp
   obtain ⟨rl', v', rr', hr1, hr2⟩ := this
   have hv: v=v_1 := by grind
   have hrnode: r = (rl.node rv rr) := by
-        apply binTreeEqR at hr
+        apply binary_tree_eq_r at hr
         simp [hr]
   constructor
-  . simp [leftAndRightAreMinHeap]
+  . simp [left_and_right_are_min_heap]
     constructor
-    . simp [isMinHeap]
+    . simp [is_min_heap]
     . specialize ih1 rl rr v_1
       simp at ih1
-      apply minHeapThenLeftAndRightAreMinHeap at hminr
-      simp [leftAndRightAreMinHeap] at hminr
+      apply min_heap_then_left_and_right_are_min_heap at hminr
+      simp [left_and_right_are_min_heap] at hminr
       simp [hrnode] at hminr
       apply ih1; all_goals grind
   . rw [hr1]
-    simp [rootIsMinOfChildren]
-    have hrvmin : f rv = heapMin (rl.node rv rr) f:= by
-      apply minHeapRootMin (rl.node rv rr) rl rr rv f (rfl)
+    simp [root_is_min_of_children]
+    have hrvmin : f rv = heap_min (rl.node rv rr) f:= by
+      apply min_heap_root_min (rl.node rv rr) rl rr rv f (rfl)
       rw[← hrnode]; exact hminr
     have hcontains: contains (node rl v_1 rr) v' := by
-      apply heapifyPreservesMembers2
+      apply heapify_contains_then_contains
       rw[hr1]
       simp[contains]
     have hcontains: contains (rl.node rv rr) v' ∨ v'= v_1 := by grind[contains]
     cases hcontains
     . expose_names
-      apply minHeapMemberLeRoot r v' at hminr
+      apply min_heap_member_le_root r v' at hminr
       rw [← hrnode] at h_1
       apply hminr at h_1
       grw[← h_1]
@@ -315,40 +313,40 @@ fun_induction heapify generalizing l r v; all_goals expose_names
     . expose_names
       rw [h_1]
       grw [h]
-. grind [isMinHeap]
+. grind [is_min_heap]
 . intro ⟨hl, hminl, hminr⟩
-  apply leftAndRightAreMinHeapAndRootIsMinOfChildrenToMinHeap
-  have: ∃ ll' v' lr', (ll.node v_1 lr).heapify f = node ll' v' lr' ∧ f v' ≤ heapMin (ll.node v_1 lr) f:= by
-        apply heapifyPreservesStructureAndRootMin
+  apply left_and_right_are_min_heap_and_root_is_min_of_children_is_min_heap
+  have: ∃ ll' v' lr', (ll.node v_1 lr).heapify f = node ll' v' lr' ∧ f v' ≤ heap_min (ll.node v_1 lr) f:= by
+        apply heapify_preserves_structure_and_root_min
         simp
   obtain ⟨rl', v', rr', hr1, hr2⟩ := this
   have hv: v=v_1 := by grind
   have hlnode: l = (ll.node lv lr) := by
-        apply binTreeEqL at hl
+        apply binary_tree_eq_l at hl
         simp [hl]
   constructor
-  . simp [leftAndRightAreMinHeap]
+  . simp [left_and_right_are_min_heap]
     constructor
     . specialize ih1 ll lr v_1
       simp at ih1
-      apply minHeapThenLeftAndRightAreMinHeap at hminl
-      simp [leftAndRightAreMinHeap] at hminl
+      apply min_heap_then_left_and_right_are_min_heap at hminl
+      simp [left_and_right_are_min_heap] at hminl
       simp [hlnode] at hminl
       apply ih1; all_goals grind
-    . simp [isMinHeap]
+    . simp [is_min_heap]
   . rw [hr1]
-    simp [rootIsMinOfChildren]
-    have hlvmin : f lv = heapMin (ll.node lv lr) f:= by
-      apply minHeapRootMin (ll.node lv lr) ll lr lv f (rfl)
+    simp [root_is_min_of_children]
+    have hlvmin : f lv = heap_min (ll.node lv lr) f:= by
+      apply min_heap_root_min (ll.node lv lr) ll lr lv f (rfl)
       rw[← hlnode]; exact hminl
     have hcontains: contains (node ll v_1 lr) v' := by
-      apply heapifyPreservesMembers2
+      apply heapify_contains_then_contains
       rw[hr1]
       simp[contains]
     have hcontains: contains (ll.node lv lr) v' ∨ v'= v_1 := by grind[contains]
     cases hcontains
     . expose_names
-      apply minHeapMemberLeRoot l v' at hminl
+      apply min_heap_member_le_root l v' at hminl
       rw [← hlnode] at h_1
       apply hminl at h_1
       grw[← h_1]
@@ -357,85 +355,85 @@ fun_induction heapify generalizing l r v; all_goals expose_names
     . expose_names
       rw [h_1]
       grw [h]
-. grind [isMinHeap]
-. grind [isMinHeap]
+. grind [is_min_heap]
+. grind [is_min_heap]
 . intro ⟨hl, hminl, hminr⟩
-  apply leftAndRightAreMinHeapAndRootIsMinOfChildrenToMinHeap
-  have: ∃ ll' v' lr', (ll.node v_1 lr).heapify f = node ll' v' lr' ∧ f v' ≤ heapMin (ll.node v_1 lr) f:= by
-        apply heapifyPreservesStructureAndRootMin
+  apply left_and_right_are_min_heap_and_root_is_min_of_children_is_min_heap
+  have: ∃ ll' v' lr', (ll.node v_1 lr).heapify f = node ll' v' lr' ∧ f v' ≤ heap_min (ll.node v_1 lr) f:= by
+        apply heapify_preserves_structure_and_root_min
         simp
   obtain ⟨rl', v', rr', hr1, hr2⟩ := this
   have hv: v=v_1 := by grind
   have hlnode: l = (ll.node lv lr) := by
-        apply binTreeEqL at hl
+        apply binary_tree_eq_l at hl
         simp [hl]
   constructor
-  . simp [leftAndRightAreMinHeap]
+  . simp [left_and_right_are_min_heap]
     constructor
     . specialize ih1 ll lr v_1
       simp at ih1
-      apply minHeapThenLeftAndRightAreMinHeap at hminl
-      simp [leftAndRightAreMinHeap] at hminl
+      apply min_heap_then_left_and_right_are_min_heap at hminl
+      simp [left_and_right_are_min_heap] at hminl
       simp [hlnode] at hminl
       apply ih1; all_goals grind
     . grind
   . rw [hr1]
-    simp [rootIsMinOfChildren]
-    have hlvmin : f lv = heapMin (ll.node lv lr) f := by
-      apply minHeapRootMin (ll.node lv lr) ll lr lv f (rfl)
+    simp [root_is_min_of_children]
+    have hlvmin : f lv = heap_min (ll.node lv lr) f := by
+      apply min_heap_root_min (ll.node lv lr) ll lr lv f (rfl)
       rw[← hlnode]; exact hminl
     have hcontains: contains (node ll v_1 lr) v' := by
-      apply heapifyPreservesMembers2
+      apply heapify_contains_then_contains
       rw[hr1]
       simp[contains]
     have hcontains: contains (ll.node lv lr) v' ∨ v'= v_1 := by grind[contains]
     cases hcontains
     . expose_names
-      apply minHeapMemberLeRoot l v' at hminl
+      apply min_heap_member_le_root l v' at hminl
       grind
     . expose_names
       grind
-. grind [isMinHeap]
+. grind [is_min_heap]
 . intro ⟨hr, hminl, hminr⟩
-  apply leftAndRightAreMinHeapAndRootIsMinOfChildrenToMinHeap
-  have: ∃ rl' v' rr', (rl.node v_1 rr).heapify f = node rl' v' rr' ∧ f v' ≤ heapMin (rl.node v_1 rr) f:= by
-        apply heapifyPreservesStructureAndRootMin
+  apply left_and_right_are_min_heap_and_root_is_min_of_children_is_min_heap
+  have: ∃ rl' v' rr', (rl.node v_1 rr).heapify f = node rl' v' rr' ∧ f v' ≤ heap_min (rl.node v_1 rr) f:= by
+        apply heapify_preserves_structure_and_root_min
         simp
   obtain ⟨rl', v', rr', hr1, hr2⟩ := this
   have hv: v=v_1 := by grind
   have hrnode: r = (rl.node rv rr) := by
-        apply binTreeEqR at hr
+        apply binary_tree_eq_r at hr
         simp [hr]
   constructor
-  . simp [leftAndRightAreMinHeap]
+  . simp [left_and_right_are_min_heap]
     constructor
     . grind
     . specialize ih1 rl rr v_1
       simp at ih1
-      apply minHeapThenLeftAndRightAreMinHeap at hminr
-      simp [leftAndRightAreMinHeap] at hminr
+      apply min_heap_then_left_and_right_are_min_heap at hminr
+      simp [left_and_right_are_min_heap] at hminr
       simp [hrnode] at hminr
       apply ih1
       . grind
       . obtain ⟨h1, h2⟩ := hminr
         exact h2
   . rw [hr1]
-    simp [rootIsMinOfChildren]
-    have hrvmin : f rv = heapMin (rl.node rv rr) f := by
-      apply minHeapRootMin (rl.node rv rr) rl rr rv f (rfl)
+    simp [root_is_min_of_children]
+    have hrvmin : f rv = heap_min (rl.node rv rr) f := by
+      apply min_heap_root_min (rl.node rv rr) rl rr rv f (rfl)
       rw[← hrnode]; exact hminr
     have hcontains: contains (node rl v_1 rr) v' := by
-      apply heapifyPreservesMembers2
+      apply heapify_contains_then_contains
       rw[hr1]
       simp[contains]
     have hcontains: contains (rl.node rv rr) v' ∨ v'= v_1 := by
-      apply containsRootOrChildren (node rl v_1 rr) rl rr v_1 v' (rfl) at hcontains
+      apply contains_root_or_children (node rl v_1 rr) rl rr v_1 v' (rfl) at hcontains
       cases hcontains; all_goals expose_names
       . left
-        apply containsLeftThenContainsRoot (node rl rv rr) rl rr rv v' (rfl) (h_2)
+        apply contains_left_then_contains_root (node rl rv rr) rl rr rv v' (rfl) (h_2)
       . cases h_2; all_goals expose_names
         . left
-          apply containsRightThenContainsRoot (node rl rv rr) rl rr rv v' (rfl) (h_2)
+          apply contains_right_then_contains_root (node rl rv rr) rl rr rv v' (rfl) (h_2)
         . right
           rw [h_2]
     constructor
@@ -443,7 +441,7 @@ fun_induction heapify generalizing l r v; all_goals expose_names
       grw [h]
     cases hcontains
     . expose_names
-      apply minHeapMemberLeRoot r v' at hminr
+      apply min_heap_member_le_root r v' at hminr
       rw [← hrnode] at h_2
       apply hminr at h_2
       grw[← h_2]
@@ -454,67 +452,70 @@ fun_induction heapify generalizing l r v; all_goals expose_names
       simp at h_1
       grw [h_1]
 
-lemma heapifyEstablishesMinHeap (bt: BinaryTree α) (f: α → ENat): (hbt: leftAndRightAreMinHeap bt f) → isMinHeap (heapify bt f) f := by
+lemma heapify_establishes_min_heap' (bt: BinaryTree α) (f: α → ENat): (hbt: left_and_right_are_min_heap bt f) → is_min_heap (heapify bt f) f := by
 cases bt
-. grind[isMinHeap,leftAndRightAreMinHeap, heapify]
-. grind[isMinHeap,leftAndRightAreMinHeap, heapifyEstablishesMinHeap']
+. grind[is_min_heap,left_and_right_are_min_heap, heapify]
+. grind[is_min_heap,left_and_right_are_min_heap, heapify_establishes_min_heap]
 
-lemma getLastPreservesMinHeap (bt: BinaryTree α) (f: α → ENat): isMinHeap bt f → isMinHeap (getLast bt).snd f := by
+theorem heapify_correctness (bt: BinaryTree α) (f: α → ENat): (contains (heapify bt f) v ↔ contains bt v) ∧  bt = node l v r ∧  is_min_heap l f ∧ is_min_heap r f → is_min_heap (heapify bt f) f := by
+grind[heapify_establishes_min_heap, contains_then_heapify_contains, heapify_contains_then_contains]
+
+lemma get_last_preserves_min_heap (bt: BinaryTree α) (f: α → ENat): is_min_heap bt f → is_min_heap (get_last bt).snd f := by
 intros; expose_names
-fun_induction isMinHeap; all_goals expose_names
+fun_induction is_min_heap; all_goals expose_names
 . grind
 . grind
-. rw [getLast]
-  apply leftAndRightAreMinHeapAndRootIsMinOfChildrenToMinHeap
+. rw [get_last]
+  apply left_and_right_are_min_heap_and_root_is_min_of_children_is_min_heap
   constructor; all_goals try grind
   . cases a; all_goals (cases a_1; all_goals grind)
-. rw [getLast]
-  apply leftAndRightAreMinHeapAndRootIsMinOfChildrenToMinHeap
+. rw [get_last]
+  apply left_and_right_are_min_heap_and_root_is_min_of_children_is_min_heap
   constructor; all_goals try grind
   . cases a; all_goals (cases a_1; all_goals grind)
-. rw [getLast]
-  apply leftAndRightAreMinHeapAndRootIsMinOfChildrenToMinHeap
+. rw [get_last]
+  apply left_and_right_are_min_heap_and_root_is_min_of_children_is_min_heap
   constructor; all_goals try grind
   . cases a; all_goals (cases a_1; all_goals grind)
 
-lemma getLastPreservesRoot (bt l r: BinaryTree α) (v v': α): bt = node l v r → bt.getLast.snd = node l' v' r' → v = v' := by
-fun_induction getLast; all_goals grind
+lemma get_last_preserves_root (bt l r: BinaryTree α) (v v': α): bt = node l v r → bt.get_last.snd = node l' v' r' → v = v' := by
+fun_induction get_last; all_goals grind
 
-lemma getLastNode (bt l r: BinaryTree α) (v: α): bt = node l v r → ∃ bt' v', (some v', bt') = getLast bt := by
+lemma get_last_is_node (bt l r: BinaryTree α) (v: α): bt = node l v r → ∃ bt' v', (some v', bt') = get_last bt := by
 intro hbt
-fun_induction getLast generalizing l v r; all_goals (expose_names; try grind)
+fun_induction get_last generalizing l v r; all_goals (expose_names; try grind)
 . cases r_1; all_goals expose_names
   . contradiction
-  . have: ∃ bt' v', (some v', bt') = (a.node a_1 a_2).getLast := by
+  . have: ∃ bt' v', (some v', bt') = (a.node a_1 a_2).get_last := by
       apply ih1 a a_2 a_1 (rfl)
     obtain ⟨bt', v', h⟩ := this
     use (node leaf v_1 bt'), v'
     grind
 . cases l_1; all_goals expose_names
   . contradiction
-  . have: ∃ bt' v', (some v', bt') = (a.node a_1 a_2).getLast := by
+  . have: ∃ bt' v', (some v', bt') = (a.node a_1 a_2).get_last := by
       apply ih1 a a_2 a_1 (rfl)
     obtain ⟨bt', v', h⟩ := this
     use (node bt' v_1 r_1), v'
     grind
 
-lemma getLastPreservesMembersExceptLast (bt l r: BinaryTree α) (v v': α): bt = node l v r → contains bt v' → (getLast bt).1 ≠ some v' → contains (getLast bt).2 v' := by
+lemma get_last_preserves_members_except_last (bt l r: BinaryTree α) (v v': α): bt = node l v r → contains bt v' → (get_last bt).1 ≠ some v' → contains (get_last bt).2 v' := by
 intros hbt hbtc hv
-fun_induction getLast generalizing l r v; all_goals (expose_names; try grind)
+fun_induction get_last generalizing l r v; all_goals (expose_names; try grind)
 . simp
   cases r_1
   . contradiction
   . expose_names
     cases a
     . cases a_2
-      . simp [getLast]
+      . simp [get_last]
         grind
-      . simp [getLast]
+      . simp [get_last]
         grind
     . cases a_2
-      . simp [getLast]
+      . simp [get_last]
         grind
-      . simp [getLast]
+      . simp [get_last]
         grind
 . simp
   cases l_1
@@ -522,21 +523,21 @@ fun_induction getLast generalizing l r v; all_goals (expose_names; try grind)
   . expose_names
     cases a
     . cases a_2
-      . simp [getLast]
+      . simp [get_last]
         grind
-      . simp [getLast]
+      . simp [get_last]
         grind
     . cases a_2
-      . simp [getLast]
+      . simp [get_last]
         grind
-      . simp [getLast]
+      . simp [get_last]
         grind
 
-lemma extractMinPreservesMembersExceptRoot (bt l r: BinaryTree α) (v: α) (f: α → ENat): bt = node l v r  → isMinHeap bt f → contains bt v' → v ≠  v' → contains (extractMin bt f).2 v' := by
+lemma extract_min_preserves_members_except_root (bt l r: BinaryTree α) (v: α) (f: α → ENat): bt = node l v r  → is_min_heap bt f → contains bt v' → v ≠  v' → contains (extract_min bt f).2 v' := by
   intros; expose_names
 
-  have hex: ∃ bt' v'', (some v'', bt') = getLast bt := by
-    apply getLastNode bt l r v h
+  have hex: ∃ bt' v'', (some v'', bt') = get_last bt := by
+    apply get_last_is_node bt l r v h
   obtain ⟨bt', v'', hv⟩ := hex
   have hlr: contains l v' ∨ contains r v' :=
     by grind
@@ -548,88 +549,88 @@ lemma extractMinPreservesMembersExceptRoot (bt l r: BinaryTree α) (v: α) (f: �
     grind
   . expose_names
     have: a_1 = v := by
-      grind[getLastPreservesRoot]
+      grind[get_last_preserves_root]
     have: a_1 ≠ v' := by grind
     have: l≠ leaf ∨ r≠leaf := by grind
     cases this; all_goals expose_names
-    . rw [extractMin]
+    . rw [extract_min]
       rw [← hv]
       simp
-      apply heapifyPreservesMembers (a.node v'' a_2) v' f
+      apply contains_then_heapify_contains (a.node v'' a_2) v' f
       by_cases v'' = v'
       . grind
-      . suffices (l.node v r).getLast.2.contains v' by grind
-        have hgl: (l.node v r).getLast.1 ≠ some v' := by grind
-        apply getLastPreservesMembersExceptLast (node l v r) l r v v' (rfl) (_) hgl
+      . suffices (l.node v r).get_last.2.contains v' by grind
+        have hgl: (l.node v r).get_last.1 ≠ some v' := by grind
+        apply get_last_preserves_members_except_last (node l v r) l r v v' (rfl) (_) hgl
         grind
-    . rw [extractMin]
+    . rw [extract_min]
       rw [← hv]
       simp
-      apply heapifyPreservesMembers (a.node v'' a_2) v' f
+      apply contains_then_heapify_contains (a.node v'' a_2) v' f
       by_cases v'' = v'
       . grind
-      . suffices (l.node v r).getLast.2.contains v' by grind
-        have hgl: (l.node v r).getLast.1 ≠ some v' := by grind
-        apply getLastPreservesMembersExceptLast (node l v r) l r v v' (rfl) (_) hgl
+      . suffices (l.node v r).get_last.2.contains v' by grind
+        have hgl: (l.node v r).get_last.1 ≠ some v' := by grind
+        apply get_last_preserves_members_except_last (node l v r) l r v v' (rfl) (_) hgl
         grind
 
-lemma extractMinCorrectNode (bt l r: BinaryTree α) (v: α) (f: α → ENat): bt = node l v r  → isMinHeap bt f → ∃ bt' v', extractMin bt f = (some v', bt') ∧ isMinHeap bt' f ∧ f v = heapMin bt f := by
+lemma extract_min_correct_node (bt l r: BinaryTree α) (v: α) (f: α → ENat): bt = node l v r  → is_min_heap bt f → ∃ bt' v', extract_min bt f = (some v', bt') ∧ is_min_heap bt' f ∧ f v = heap_min bt f := by
   intros; expose_names
-  have hex: ∃ bt' v'', (some v'', bt') = getLast bt := by
-    apply getLastNode bt l r v h
+  have hex: ∃ bt' v'', (some v'', bt') = get_last bt := by
+    apply get_last_is_node bt l r v h
   obtain ⟨bt', v'', hv⟩ := hex
   cases bt'
   . use leaf
     use v''
-    grind [isMinHeap, minHeapRootMin]
+    grind [is_min_heap, min_heap_root_min]
   . expose_names
     use (heapify (node a v'' a_2) f)
     use v
     constructor
-    . rw [extractMin.eq_1]
+    . rw [extract_min.eq_1]
       simp [← hv]
-      grind [getLastPreservesRoot]
+      grind [get_last_preserves_root]
     . constructor
-      . have: isMinHeap (node a a_1 a_2) f := by grind[getLastPreservesMinHeap]
-        apply minHeapThenLeftAndRightAreMinHeap at this
-        grind [leftAndRightAreMinHeap, heapifyEstablishesMinHeap]
-      . grind [minHeapRootMin]
+      . have: is_min_heap (node a a_1 a_2) f := by grind[get_last_preserves_min_heap]
+        apply min_heap_then_left_and_right_are_min_heap at this
+        grind [left_and_right_are_min_heap, heapify_establishes_min_heap']
+      . grind [min_heap_root_min]
 
-lemma getLastReturnsSome {α : Type u} [DecidableEq α] (bt : BinaryTree α) (hbt: bt ≠ leaf): ∃ v, some v = (getLast bt).1 := by
-fun_induction getLast; all_goals grind
+lemma get_last_returns_some {α : Type u} [DecidableEq α] (bt : BinaryTree α) (hbt: bt ≠ leaf): ∃ v, some v = (get_last bt).1 := by
+fun_induction get_last; all_goals grind
 
-lemma extractMinReturnsSome {α : Type u} [DecidableEq α] (bt : BinaryTree α) (f : α → ENat) (hbt: bt ≠ leaf): ∃ v, some v = (extractMin bt f).1 := by
-have: ∃ v, some v = (getLast bt).1 := by apply getLastReturnsSome bt hbt
+lemma extract_min_returns_some {α : Type u} [DecidableEq α] (bt : BinaryTree α) (f : α → ENat) (hbt: bt ≠ leaf): ∃ v, some v = (extract_min bt f).1 := by
+have: ∃ v, some v = (get_last bt).1 := by apply get_last_returns_some bt hbt
 grind
 
-lemma extractMinIsSome {α : Type u} [DecidableEq α] (bt : BinaryTree α) (f : α → ENat) (hbt: bt ≠ leaf):(extractMin bt f).1.isSome := by
-have: ∃ v, some v = (getLast bt).1 := by apply getLastReturnsSome bt hbt
+lemma extract_min_is_some {α : Type u} [DecidableEq α] (bt : BinaryTree α) (f : α → ENat) (hbt: bt ≠ leaf):(extract_min bt f).1.isSome := by
+have: ∃ v, some v = (get_last bt).1 := by apply get_last_returns_some bt hbt
 grind
 
-lemma insertIsNode (bt: BinaryTree α) (f: α → ENat) (v: α): ∃ l r v', insert bt v f = node l v' r := by
+lemma insert_is_node (bt: BinaryTree α) (f: α → ENat) (v: α): ∃ l r v', insert bt v f = node l v' r := by
 fun_induction insert
 . grind
 . grind
 . grind
 
-lemma insertThenContains (bt: BinaryTree α) (v: α) (f: α → ENat): contains (insert bt v f) v := by
+lemma insert_then_contains (bt: BinaryTree α) (v: α) (f: α → ENat): contains (insert bt v f) v := by
 fun_induction insert; all_goals grind
 
-lemma insertContainsnOldMemberOrNewValue (bt: BinaryTree α) (v v': α) (f: α → ENat): contains (insert bt v f) v' → contains bt v' ∨ v = v' := by
+lemma insert_then_insert_contains_old_member_or_new_value_contains (bt: BinaryTree α) (v v': α) (f: α → ENat): contains (insert bt v f) v' → contains bt v' ∨ v = v' := by
 intro hbt
 fun_induction insert; all_goals grind
 
-lemma insertPreservesMinHeap (bt: BinaryTree α) (v: α) (f: α → ENat): isMinHeap bt f → isMinHeap (insert bt v f) f := by
+lemma insert_preserves_min_heap (bt: BinaryTree α) (v: α) (f: α → ENat): is_min_heap bt f → is_min_heap (insert bt v f) f := by
 intro hbt
 have hbtp := hbt
 fun_induction insert
 . grind
 . expose_names
-  apply leftAndRightAreMinHeapAndRootIsMinOfChildrenToMinHeap
-  apply minHeapThenLeftAndRightAreMinHeap at hbt
-  simp [leftAndRightAreMinHeap] at hbt
+  apply left_and_right_are_min_heap_and_root_is_min_of_children_is_min_heap
+  apply min_heap_then_left_and_right_are_min_heap at hbt
+  simp [left_and_right_are_min_heap] at hbt
   constructor
-  . simp [leftAndRightAreMinHeap]
+  . simp [left_and_right_are_min_heap]
     constructor
     . apply ih1
       grind
@@ -637,46 +638,46 @@ fun_induction insert
       exact hl
     . simp [hbt]
   . cases r
-    . obtain ⟨l', r', v', h' ⟩ := insertIsNode l f v_1
+    . obtain ⟨l', r', v', h' ⟩ := insert_is_node l f v_1
       rw [h']
-      simp [rootIsMinOfChildren]
+      simp [root_is_min_of_children]
       have: contains l v' ∨ v_1 = v' := by
-        apply insertContainsnOldMemberOrNewValue l v_1 v' f
+        apply insert_then_insert_contains_old_member_or_new_value_contains l v_1 v' f
         rw [h']
         grind
       cases this
       . expose_names
         obtain ⟨hl, hr⟩ := hbt
         grw [h]
-        apply minHeapThenMembersLeftLe (l.node v_1 leaf) l leaf v_1 v' f hbtp (rfl) h_1
+        apply min_heap_then_members_left_le (l.node v_1 leaf) l leaf v_1 v' f hbtp (rfl) h_1
       . expose_names
         rw [←h_1]
         exact h
     . expose_names
-      obtain ⟨l', r', v', h' ⟩ := insertIsNode l f v_1
+      obtain ⟨l', r', v', h' ⟩ := insert_is_node l f v_1
       rw [h']
-      simp [rootIsMinOfChildren]
+      simp [root_is_min_of_children]
       constructor
       . have: contains l v' ∨ v_1 = v' := by
-          apply insertContainsnOldMemberOrNewValue l v_1 v' f
+          apply insert_then_insert_contains_old_member_or_new_value_contains l v_1 v' f
           rw [h']
           grind
         cases this
         . expose_names
           obtain ⟨hl, hr⟩ := hbt
           grw [h]
-          apply minHeapThenMembersLeftLe (l.node v_1 (a.node a_1 a_2)) l (a.node a_1 a_2) v_1 v' f hbtp (rfl) h_1
+          apply min_heap_then_members_left_le (l.node v_1 (a.node a_1 a_2)) l (a.node a_1 a_2) v_1 v' f hbtp (rfl) h_1
         . expose_names
           rw [←h_1]
           exact h
       . grw [h]
-        apply minHeapThenMembersRightLe (l.node v_1 (a.node a_1 a_2)) l (a.node a_1 a_2) v_1 a_1 f hbtp (rfl) (by grind)
+        apply min_heap_then_members_right_le (l.node v_1 (a.node a_1 a_2)) l (a.node a_1 a_2) v_1 a_1 f hbtp (rfl) (by grind)
 . expose_names
-  apply leftAndRightAreMinHeapAndRootIsMinOfChildrenToMinHeap
-  apply minHeapThenLeftAndRightAreMinHeap at hbt
-  simp [leftAndRightAreMinHeap] at hbt
+  apply left_and_right_are_min_heap_and_root_is_min_of_children_is_min_heap
+  apply min_heap_then_left_and_right_are_min_heap at hbt
+  simp [left_and_right_are_min_heap] at hbt
   constructor
-  . simp [leftAndRightAreMinHeap]
+  . simp [left_and_right_are_min_heap]
     constructor
     . apply ih1
       grind
@@ -684,41 +685,41 @@ fun_induction insert
       exact hl
     . simp [hbt]
   . cases r
-    . obtain ⟨l', r', v', h' ⟩ := insertIsNode l f v
+    . obtain ⟨l', r', v', h' ⟩ := insert_is_node l f v
       rw [h']
-      simp [rootIsMinOfChildren]
+      simp [root_is_min_of_children]
       have: contains l v' ∨ v = v' := by
-        apply insertContainsnOldMemberOrNewValue l v v' f
+        apply insert_then_insert_contains_old_member_or_new_value_contains l v v' f
         rw [h']
         grind
       cases this
       . expose_names
         obtain ⟨hl, hr⟩ := hbt
-        apply minHeapThenMembersLeftLe (l.node v_1 leaf) l leaf v_1 v' f  hbtp (rfl) h_1
+        apply min_heap_then_members_left_le (l.node v_1 leaf) l leaf v_1 v' f  hbtp (rfl) h_1
       . expose_names
         rw [←h_1]
         simp at h
         grw [h]
     . expose_names
-      obtain ⟨l', r', v', h' ⟩ := insertIsNode l f v
+      obtain ⟨l', r', v', h' ⟩ := insert_is_node l f v
       rw [h']
-      simp [rootIsMinOfChildren]
+      simp [root_is_min_of_children]
       constructor
       . have: contains l v' ∨ v = v' := by
-          apply insertContainsnOldMemberOrNewValue l v v' f
+          apply insert_then_insert_contains_old_member_or_new_value_contains l v v' f
           rw [h']
           grind
         cases this
         . expose_names
           obtain ⟨hl, hr⟩ := hbt
-          apply minHeapThenMembersLeftLe (l.node v_1 (a.node a_1 a_2)) l (a.node a_1 a_2) v_1 v' f hbtp (rfl) h_1
+          apply min_heap_then_members_left_le (l.node v_1 (a.node a_1 a_2)) l (a.node a_1 a_2) v_1 v' f hbtp (rfl) h_1
         . expose_names
           rw [←h_1]
           simp at h
           grw [h]
-      . apply minHeapThenMembersRightLe (l.node v_1 (a.node a_1 a_2)) l (a.node a_1 a_2) v_1 a_1 f hbtp (rfl) (by grind)
+      . apply min_heap_then_members_right_le (l.node v_1 (a.node a_1 a_2)) l (a.node a_1 a_2) v_1 a_1 f hbtp (rfl) (by grind)
 
-lemma insertPreservesExistingMembers (bt: BinaryTree α) (v v': α) (f: α → ENat): contains bt v →  contains (insert bt v' f) v := by
+lemma insert_preserves_existing_members (bt: BinaryTree α) (v v': α) (f: α → ENat): contains bt v →  contains (insert bt v' f) v := by
 intro hbt
 fun_induction insert; all_goals expose_names
 . contradiction
@@ -729,7 +730,7 @@ fun_induction insert; all_goals expose_names
     right
     left
     rw [h_1]
-    grind [insertThenContains]
+    grind [insert_then_contains]
   . expose_names
     cases h_1; all_goals expose_names
     . simp [contains]
@@ -779,24 +780,24 @@ fun_induction insert; all_goals expose_names
       else
         node (remove l x f) v (remove r x f)
 
-@[grind] def decreasePriority [DecidableEq α] (bt : BinaryTree α) (v : α) (f : α → ENat): BinaryTree α :=
-  if containsB bt v then insert (remove bt v f) v f else bt
+@[grind] def decrease_priority [DecidableEq α] (bt : BinaryTree α) (v : α) (f : α → ENat): BinaryTree α :=
+  if containsb bt v then insert (remove bt v f) v f else bt
 
-lemma mergeLeftIdNodeIsNode (bt1 bt2 l1 r1: BinaryTree α) (f: α → ENat) (v1: α): bt1 = node l1 v1 r1 → ∃ l v r, merge bt1 bt2 f = node l v r := by
+lemma merge_left_is_node_is_node (bt1 bt2 l1 r1: BinaryTree α) (f: α → ENat) (v1: α): bt1 = node l1 v1 r1 → ∃ l v r, merge bt1 bt2 f = node l v r := by
 fun_induction merge
 . grind
 . grind
 . grind
 . grind
 
-lemma mergeRightIdNodeIsNode (bt1 bt2 l2 r2: BinaryTree α) (f: α → ENat) (v2: α): bt2 = node l2 v2 r2 → ∃ l v r, merge bt1 bt2 f = node l v r := by
+lemma merge_right_is_node_is_node (bt1 bt2 l2 r2: BinaryTree α) (f: α → ENat) (v2: α): bt2 = node l2 v2 r2 → ∃ l v r, merge bt1 bt2 f = node l v r := by
 fun_induction merge
 . grind
 . grind
 . grind
 . grind
 
-lemma mergeLeftContains (bt1 l1 r1 bt2 l r: BinaryTree α) (v1 v: α ) (f: α → ENat): (merge bt1 bt2 f) = node l v r → isMinHeap bt1 f → isMinHeap bt2 f →  bt1 = node l1 v1 r1 → contains bt2 v ∨ v = v1 := by
+lemma merge_left_contains (bt1 l1 r1 bt2 l r: BinaryTree α) (v1 v: α ) (f: α → ENat): (merge bt1 bt2 f) = node l v r → is_min_heap bt1 f → is_min_heap bt2 f →  bt1 = node l1 v1 r1 → contains bt2 v ∨ v = v1 := by
 intro h
 fun_induction merge generalizing l1 r1 v1
 . grind
@@ -809,7 +810,7 @@ fun_induction merge generalizing l1 r1 v1
 . expose_names
   grind
 
-lemma mergeRightContains (bt1 l2 r2 bt2 l r: BinaryTree α) (v2 v: α ) (f: α → ENat): (merge bt1 bt2 f) = node l v r → isMinHeap bt1 f → isMinHeap bt2 f →  bt2 = node l2 v2 r2 → contains bt1 v ∨ v = v2 := by
+lemma merge_right_contains (bt1 l2 r2 bt2 l r: BinaryTree α) (v2 v: α ) (f: α → ENat): (merge bt1 bt2 f) = node l v r → is_min_heap bt1 f → is_min_heap bt2 f →  bt2 = node l2 v2 r2 → contains bt1 v ∨ v = v2 := by
 intro h
 fun_induction merge generalizing l2 r2 v2
 . grind
@@ -822,166 +823,166 @@ fun_induction merge generalizing l2 r2 v2
 . expose_names
   grind
 
-lemma mergePreservesMinHeap (bt1 bt2 : BinaryTree α) (f : α → ENat) (h1 : isMinHeap bt1 f) (h2 : isMinHeap bt2 f) : isMinHeap (merge bt1 bt2 f) f := by
+lemma merge_preserves_min_heap (bt1 bt2 : BinaryTree α) (f : α → ENat) (h1 : is_min_heap bt1 f) (h2 : is_min_heap bt2 f) : is_min_heap (merge bt1 bt2 f) f := by
 fun_induction merge
 . grind
 . grind
 . expose_names
-  apply leftAndRightAreMinHeapAndRootIsMinOfChildrenToMinHeap
+  apply left_and_right_are_min_heap_and_root_is_min_of_children_is_min_heap
   constructor
   . constructor
     . apply ih1
-      apply minHeapThenLeftAndRightAreMinHeap at h1
-      simp [leftAndRightAreMinHeap] at h1
+      apply min_heap_then_left_and_right_are_min_heap at h1
+      simp [left_and_right_are_min_heap] at h1
       obtain ⟨ hl, hr ⟩ := h1
       exact hl
       exact h2
-    . apply minHeapThenLeftAndRightAreMinHeap at h1
-      simp [leftAndRightAreMinHeap] at h1
+    . apply min_heap_then_left_and_right_are_min_heap at h1
+      simp [left_and_right_are_min_heap] at h1
       obtain ⟨ hl, hr ⟩ := h1
       exact hr
-  . obtain ⟨ l, v, r, hr ⟩ := mergeRightIdNodeIsNode l1 (l2.node v2 r2) l2 r2 f v2 (rfl)
+  . obtain ⟨ l, v, r, hr ⟩ := merge_right_is_node_is_node l1 (l2.node v2 r2) l2 r2 f v2 (rfl)
     rw [hr]
     cases r1
-    . simp[rootIsMinOfChildren]
+    . simp[root_is_min_of_children]
       have: contains l1 v ∨ v = v2 := by
-        apply mergeRightContains l1 l2 r2 (l2.node v2 r2) l r v2 v f hr _ h2 (rfl)
-        apply minHeapThenLeftAndRightAreMinHeap at h1
-        simp [leftAndRightAreMinHeap] at h1
+        apply merge_right_contains l1 l2 r2 (l2.node v2 r2) l r v2 v f hr _ h2 (rfl)
+        apply min_heap_then_left_and_right_are_min_heap at h1
+        simp [left_and_right_are_min_heap] at h1
         simp [h1]
       cases this
-      . apply minHeapThenMembersLeftLe (l1.node v1 leaf) l1 leaf v1 v f h1 (rfl) (by grind)
+      . apply min_heap_then_members_left_le (l1.node v1 leaf) l1 leaf v1 v f h1 (rfl) (by grind)
       . expose_names
         rw [h_1]
         exact h
-    . simp[rootIsMinOfChildren]
+    . simp[root_is_min_of_children]
       have: contains l1 v ∨ v = v2 := by
-        apply mergeRightContains l1 l2 r2 (l2.node v2 r2) l r v2 v f hr _ h2 (rfl)
-        apply minHeapThenLeftAndRightAreMinHeap at h1
-        simp [leftAndRightAreMinHeap] at h1
+        apply merge_right_contains l1 l2 r2 (l2.node v2 r2) l r v2 v f hr _ h2 (rfl)
+        apply min_heap_then_left_and_right_are_min_heap at h1
+        simp [left_and_right_are_min_heap] at h1
         simp [h1]
       cases this
       . expose_names
         constructor
-        . apply minHeapThenMembersLeftLe (l1.node v1 (a.node a_1 a_2)) l1 (a.node a_1 a_2) v1 v f h1 (rfl) (by grind)
-        . apply minHeapThenMembersRightLe (l1.node v1 (a.node a_1 a_2)) l1 (a.node a_1 a_2) v1 a_1 f h1 (rfl) (by grind)
+        . apply min_heap_then_members_left_le (l1.node v1 (a.node a_1 a_2)) l1 (a.node a_1 a_2) v1 v f h1 (rfl) (by grind)
+        . apply min_heap_then_members_right_le (l1.node v1 (a.node a_1 a_2)) l1 (a.node a_1 a_2) v1 a_1 f h1 (rfl) (by grind)
       . expose_names
         rw [h_1]
         constructor
         . exact h
-        . apply minHeapThenMembersRightLe (l1.node v1 (a.node a_1 a_2)) l1 (a.node a_1 a_2) v1 a_1 f h1 (rfl) (by grind)
+        . apply min_heap_then_members_right_le (l1.node v1 (a.node a_1 a_2)) l1 (a.node a_1 a_2) v1 a_1 f h1 (rfl) (by grind)
 . expose_names
-  apply leftAndRightAreMinHeapAndRootIsMinOfChildrenToMinHeap
+  apply left_and_right_are_min_heap_and_root_is_min_of_children_is_min_heap
   constructor
   . constructor
     . apply ih1 h1
-      apply minHeapThenLeftAndRightAreMinHeap at h2
-      simp [leftAndRightAreMinHeap] at h2
+      apply min_heap_then_left_and_right_are_min_heap at h2
+      simp [left_and_right_are_min_heap] at h2
       obtain ⟨ hl, hr ⟩ := h2
       exact hl
-    . apply minHeapThenLeftAndRightAreMinHeap at h2
-      simp [leftAndRightAreMinHeap] at h2
+    . apply min_heap_then_left_and_right_are_min_heap at h2
+      simp [left_and_right_are_min_heap] at h2
       obtain ⟨ hl, hr ⟩ := h2
       exact hr
-  . obtain ⟨ l, v, r, hl ⟩ := mergeLeftIdNodeIsNode (l1.node v1 r1) l2 l1 r1 f v1 (rfl)
+  . obtain ⟨ l, v, r, hl ⟩ := merge_left_is_node_is_node (l1.node v1 r1) l2 l1 r1 f v1 (rfl)
     rw [hl]
     cases r2
-    . simp[rootIsMinOfChildren]
+    . simp[root_is_min_of_children]
       have: contains l2 v ∨ v = v1 := by
-        apply mergeLeftContains (l1.node v1 r1) l1 r1 l2 l r v1 v f hl h1 _ (rfl)
-        apply minHeapThenLeftAndRightAreMinHeap at h2
-        simp [leftAndRightAreMinHeap] at h2
+        apply merge_left_contains (l1.node v1 r1) l1 r1 l2 l r v1 v f hl h1 _ (rfl)
+        apply min_heap_then_left_and_right_are_min_heap at h2
+        simp [left_and_right_are_min_heap] at h2
         simp [h2]
       cases this
-      . apply minHeapThenMembersLeftLe (l2.node v2 leaf) l2 leaf v2 v f h2 (rfl) (by grind)
+      . apply min_heap_then_members_left_le (l2.node v2 leaf) l2 leaf v2 v f h2 (rfl) (by grind)
       . expose_names
         rw [h_1]
         simp at h
         grw [h]
-    . simp[rootIsMinOfChildren]
+    . simp[root_is_min_of_children]
       have: contains l2 v ∨ v = v1 := by
-        apply mergeLeftContains (l1.node v1 r1) l1 r1 l2 l r v1 v f hl h1 _ (rfl)
-        apply minHeapThenLeftAndRightAreMinHeap at h2
-        simp [leftAndRightAreMinHeap] at h2
+        apply merge_left_contains (l1.node v1 r1) l1 r1 l2 l r v1 v f hl h1 _ (rfl)
+        apply min_heap_then_left_and_right_are_min_heap at h2
+        simp [left_and_right_are_min_heap] at h2
         simp [h2]
       cases this
       . expose_names
         constructor
-        . apply minHeapThenMembersLeftLe (l2.node v2 (a.node a_1 a_2)) l2 (a.node a_1 a_2) v2 v f h2 (rfl) h_1
-        . apply minHeapThenMembersRightLe (l2.node v2 (a.node a_1 a_2)) l2 (a.node a_1 a_2) v2 a_1 f h2 (rfl) (by grind)
+        . apply min_heap_then_members_left_le (l2.node v2 (a.node a_1 a_2)) l2 (a.node a_1 a_2) v2 v f h2 (rfl) h_1
+        . apply min_heap_then_members_right_le (l2.node v2 (a.node a_1 a_2)) l2 (a.node a_1 a_2) v2 a_1 f h2 (rfl) (by grind)
       . expose_names
         rw [h_1]
         constructor
         . simp at h
           grw [h]
-        . apply minHeapThenMembersRightLe (l2.node v2 (a.node a_1 a_2)) l2 (a.node a_1 a_2) v2 a_1 f h2 (rfl) (by grind)
+        . apply min_heap_then_members_right_le (l2.node v2 (a.node a_1 a_2)) l2 (a.node a_1 a_2) v2 a_1 f h2 (rfl) (by grind)
 
-lemma mergeNoNewMembers  (bt1 bt2 : BinaryTree α) (f : α → ENat): merge bt1 bt2 f = node l v r → contains bt1 v ∨ contains bt2 v := by
+lemma merge_no_new_members  (bt1 bt2 : BinaryTree α) (f : α → ENat): merge bt1 bt2 f = node l v r → contains bt1 v ∨ contains bt2 v := by
 fun_induction merge
 . grind
 . grind
 . grind
 . grind
 
-lemma removeNoNewMembers [DecidableEq α] (bt l r : BinaryTree α) (x v: α) (f: α → ENat): bt.remove x f = node l v r → contains bt v:= by
+lemma remove_no_new_members [DecidableEq α] (bt l r : BinaryTree α) (x v: α) (f: α → ENat): bt.remove x f = node l v r → contains bt v:= by
 fun_induction remove
 . grind
 . intros
   expose_names
-  grind[mergeNoNewMembers]
-. grind[mergeNoNewMembers]
+  grind[merge_no_new_members]
+. grind[merge_no_new_members]
 
-lemma removePreservesMinHeap [DecidableEq α] (bt : BinaryTree α) (x : α) (f : α → ENat): isMinHeap bt f → isMinHeap (remove bt x f) f := by
+lemma remove_preserves_min_heap [DecidableEq α] (bt : BinaryTree α) (x : α) (f : α → ENat): is_min_heap bt f → is_min_heap (remove bt x f) f := by
 intro hmin
 fun_induction remove
 . exact hmin
 . expose_names
-  apply minHeapThenLeftAndRightAreMinHeap at hmin
-  grind [mergePreservesMinHeap]
+  apply min_heap_then_left_and_right_are_min_heap at hmin
+  grind [merge_preserves_min_heap]
 . expose_names
-  apply leftAndRightAreMinHeapAndRootIsMinOfChildrenToMinHeap
+  apply left_and_right_are_min_heap_and_root_is_min_of_children_is_min_heap
   constructor
-  simp[leftAndRightAreMinHeap]
+  simp[left_and_right_are_min_heap]
   constructor
   . apply ih2
-    apply minHeapThenLeftAndRightAreMinHeap at hmin
-    simp[leftAndRightAreMinHeap] at hmin
+    apply min_heap_then_left_and_right_are_min_heap at hmin
+    simp[left_and_right_are_min_heap] at hmin
     simp_all
   . apply ih1
-    apply minHeapThenLeftAndRightAreMinHeap at hmin
-    simp[leftAndRightAreMinHeap] at hmin
+    apply min_heap_then_left_and_right_are_min_heap at hmin
+    simp[left_and_right_are_min_heap] at hmin
     simp_all
   . cases hl : l.remove x f with
     | leaf =>
         cases hr : r.remove x f with
         | leaf =>
-          simp[rootIsMinOfChildren]
+          simp[root_is_min_of_children]
         | node l'' v'' r'' =>
-          simp[rootIsMinOfChildren]
-          have: contains r v'' := by grind[removeNoNewMembers]
-          apply minHeapThenMembersRightLe (l.node v r) l r v v'' f hmin (rfl) this
+          simp[root_is_min_of_children]
+          have: contains r v'' := by grind[remove_no_new_members]
+          apply min_heap_then_members_right_le (l.node v r) l r v v'' f hmin (rfl) this
     | node l' v' r' =>
         cases hr : r.remove x f with
         | leaf =>
-          simp[rootIsMinOfChildren]
-          have: contains l v' := by grind[removeNoNewMembers]
-          apply minHeapThenMembersLeftLe (l.node v r) l r v v' f hmin (rfl) this
+          simp[root_is_min_of_children]
+          have: contains l v' := by grind[remove_no_new_members]
+          apply min_heap_then_members_left_le (l.node v r) l r v v' f hmin (rfl) this
         | node l'' v'' r'' =>
-          simp[rootIsMinOfChildren]
+          simp[root_is_min_of_children]
           constructor
-          . have: contains l v' := by grind[removeNoNewMembers]
-            apply minHeapThenMembersLeftLe (l.node v r) l r v v' f hmin (rfl) this
-          . have: contains r v'' := by grind[removeNoNewMembers]
-            apply minHeapThenMembersRightLe (l.node v r) l r v v'' f hmin (rfl) this
+          . have: contains l v' := by grind[remove_no_new_members]
+            apply min_heap_then_members_left_le (l.node v r) l r v v' f hmin (rfl) this
+          . have: contains r v'' := by grind[remove_no_new_members]
+            apply min_heap_then_members_right_le (l.node v r) l r v v'' f hmin (rfl) this
 
-theorem decreasePriorityPreservesMinHeap [DecidableEq α]  (bt: BinaryTree α) (v : α) (f : α → ENat): isMinHeap bt f → isMinHeap (decreasePriority bt v f) f := by
+theorem decrease_priority_preserves_min_heap [DecidableEq α]  (bt: BinaryTree α) (v : α) (f : α → ENat): is_min_heap bt f → is_min_heap (decrease_priority bt v f) f := by
 intro hmin
-simp [decreasePriority]
-by_cases (bt.containsB v)
+simp [decrease_priority]
+by_cases (bt.containsb v)
 . expose_names
   simp [h]
-  apply insertPreservesMinHeap
-  apply removePreservesMinHeap
+  apply insert_preserves_min_heap
+  apply remove_preserves_min_heap
   exact hmin
 . expose_names
   simp [h]
@@ -991,29 +992,29 @@ def size: (BinaryTree α) →  Nat
 | leaf => 0
 | node l _ r => 1 + size l + size r
 
-@[simp] lemma sizeGeZero: size bt ≥ 0 := by
+@[simp] lemma size_ge_zero: size bt ≥ 0 := by
 fun_induction size
 . simp
 . simp
 
-lemma mergeSize [DecidableEq α] (bt1 bt2: BinaryTree α) (f : α → ENat): size (merge bt1 bt2 f) = size bt1 + size bt2 := by
+lemma merge_size [DecidableEq α] (bt1 bt2: BinaryTree α) (f : α → ENat): size (merge bt1 bt2 f) = size bt1 + size bt2 := by
 fun_induction merge
 . simp[size]
 . simp [size]
 . grind [size]
 . grind [size]
 
-lemma removeSizeDec [DecidableEq α] (bt : BinaryTree α) (v : α) (f : α → ENat) : size (remove bt v f) ≤ size bt := by
+lemma remove_size_dec [DecidableEq α] (bt : BinaryTree α) (v : α) (f : α → ENat) : size (remove bt v f) ≤ size bt := by
 fun_induction remove
 . simp
-. grind [size, mergeSize]
-. grind [size, mergeSize]
+. grind [size, merge_size]
+. grind [size, merge_size]
 
-lemma removeSize [DecidableEq α] (bt : BinaryTree α) (v : α) (f : α → ENat) (h: contains bt v): size (remove bt v f) + 1 ≤ size bt:= by
+lemma remove_size [DecidableEq α] (bt : BinaryTree α) (v : α) (f : α → ENat) (h: contains bt v): size (remove bt v f) + 1 ≤ size bt:= by
 fun_induction remove
 . contradiction
 . expose_names
-  rw [mergeSize l r f]
+  rw [merge_size l r f]
   nth_rw 3 [size.eq_def]
   simp
   grind
@@ -1027,20 +1028,20 @@ fun_induction remove
       simp[size]
       apply ih2 at h
       grw [← h]
-      grind[removeSizeDec]
+      grind[remove_size_dec]
     . expose_names
       simp [size]
       apply ih1 at h
       grw [← h]
-      grind[removeSizeDec]
+      grind[remove_size_dec]
 
-lemma insertSize [DecidableEq α] (bt : BinaryTree α) (v : α) (f : α → ENat): size (insert bt v f) = size bt + 1 := by
+lemma insert_size [DecidableEq α] (bt : BinaryTree α) (v : α) (f : α → ENat): size (insert bt v f) = size bt + 1 := by
 fun_induction insert
 . simp[size]
 . grind [size]
 . grind [size]
 
-lemma containsBSize [DecidableEq α] (bt:BinaryTree α): containsB bt v = true → bt.size ≥ 1 := by
+lemma containsb_size [DecidableEq α] (bt:BinaryTree α): containsb bt v = true → bt.size ≥ 1 := by
 cases bt
 . intro
   by_contra
@@ -1049,25 +1050,25 @@ cases bt
   simp[size]
   omega
 
-lemma containsBContains [DecidableEq α] (bt: BinaryTree α): containsB bt v → contains bt v := by
+lemma containsb_contains [DecidableEq α] (bt: BinaryTree α): containsb bt v → contains bt v := by
 intro
 fun_induction contains
 . contradiction
 . grind
 
-lemma decreasePrioritySize [DecidableEq α] (bt : BinaryTree α) (v : α) (f : α → ENat): size (decreasePriority bt v f) ≤ size bt := by
-simp[decreasePriority]
-by_cases bt.containsB v
+lemma decrease_priority_size [DecidableEq α] (bt : BinaryTree α) (v : α) (f : α → ENat): size (decrease_priority bt v f) ≤ size bt := by
+simp[decrease_priority]
+by_cases bt.containsb v
 . expose_names
   simp [h]
-  rw [insertSize]
-  grw [removeSize]
-  grind [containsBContains]
+  rw [insert_size]
+  grw [remove_size]
+  grind [containsb_contains]
 . expose_names
   simp [h]
 
-lemma getLastSize (h: bt ≠ leaf): size (getLast bt).2 < size bt := by
-fun_induction getLast
+lemma get_last_size (h: bt ≠ leaf): size (get_last bt).2 < size bt := by
+fun_induction get_last
 . contradiction
 . simp [size]
 . expose_names
@@ -1079,30 +1080,30 @@ fun_induction getLast
   apply ih1
   grind
 
-lemma heapifySize: size (heapify bt f) = size bt := by
+lemma heapify_size: size (heapify bt f) = size bt := by
 fun_induction heapify; all_goals grind [size]
 
-lemma extractMinSize (h: bt ≠ leaf): size (extractMin bt f).2 < size bt := by
+lemma extract_min_size (h: bt ≠ leaf): size (extract_min bt f).2 < size bt := by
 induction bt
 . contradiction
 . expose_names
-  have hex: ∃ bt' v'', (some v'', bt') = getLast  (a.node a_1 a_2):= by
-    apply getLastNode (a.node a_1 a_2) a a_2 a_1 (rfl)
+  have hex: ∃ bt' v'', (some v'', bt') = get_last  (a.node a_1 a_2):= by
+    apply get_last_is_node (a.node a_1 a_2) a a_2 a_1 (rfl)
   obtain ⟨bt, v, hv⟩ := hex
-  simp[extractMin]
+  simp[extract_min]
   rw[← hv]
   simp
   cases bt
   . simp[size]
   . expose_names
     simp
-    simp[heapifySize]
+    simp[heapify_size]
     have: (a_3.node v a_5).size = (a_3.node a_4 a_5).size := by simp [size]
     rw [this]
-    have: (a_3.node a_4 a_5) = (a.node a_1 a_2).getLast.2 := by
+    have: (a_3.node a_4 a_5) = (a.node a_1 a_2).get_last.2 := by
       rw [←hv]
     rw [this]
-    apply getLastSize h
+    apply get_last_size h
 
 structure BinaryHeap (α : Type u) [DecidableEq α] where
   tree : BinaryTree α
@@ -1110,6 +1111,10 @@ structure BinaryHeap (α : Type u) [DecidableEq α] where
 namespace BinaryHeap
 
 def empty [DecidableEq α]: BinaryHeap α := { tree := BinaryTree.leaf }
+
+def is_empty_tree [DecidableEq α] (bt: BinaryTree α): Bool :=  match bt with
+| leaf => true
+| node _ _ _ => false
 
 def isEmpty [DecidableEq α] (h: BinaryHeap α): Bool :=  match h.tree with
 | leaf => true
@@ -1128,23 +1133,23 @@ cases h: bh.tree
   expose_names
   simp
 
-lemma extractMinIsSomeHeap {α : Type u} [DecidableEq α] (h : BinaryHeap α) (f : α → ENat) (hh: ¬ isEmpty h): (extractMin h.tree f).1.isSome := by
-grind[isEmpty, extractMinIsSome]
+lemma extract_min_is_someHeap {α : Type u} [DecidableEq α] (h : BinaryHeap α) (f : α → ENat) (hh: ¬ isEmpty h): (extract_min h.tree f).1.isSome := by
+grind[isEmpty, extract_min_is_some]
 
 noncomputable def extract_min {α : Type u} [Nonempty α] [DecidableEq α] (h : BinaryHeap α) (priority : α → ENat) (hh: ¬ isEmpty h): (α × BinaryHeap α) :=
-  ((h.tree.extractMin priority).1.get (by grind[extractMinIsSomeHeap]) , {tree:= (h.tree.extractMin priority).2})
+  ((h.tree.extract_min priority).1.get (by grind[extract_min_is_someHeap]) , {tree:= (h.tree.extract_min priority).2})
 
 def sizeOf {α : Type u} [DecidableEq α] (h : BinaryHeap α) : Nat := h.tree.size
 
 def decrease_priority [DecidableEq α] (h : BinaryHeap α) (v : α) (prio :α →  ENat) : BinaryHeap α :=
-{tree:= decreasePriority h.tree v prio}
+{tree:= BinaryTree.decrease_priority h.tree v prio}
 
 -- Helper lemma: decreasing priority does not increase heap size
 theorem sizeOf_decrease_priority_le {α : Type u} [DecidableEq α] (h : BinaryHeap α) (v : α) (prio :α → ENat) :
   sizeOf (decrease_priority h v prio) ≤ sizeOf h := by
   -- To be proved from the concrete heap implementation
   simp [decrease_priority, sizeOf]
-  grind[decreasePrioritySize]
+  grind[decrease_priority_size]
 
 -- Helper lemma: extracting the minimum from a non-empty heap strictly decreases its size.
 theorem sizeOf_extract_min_lt_of_isEmpty_eq_false
@@ -1153,9 +1158,41 @@ theorem sizeOf_extract_min_lt_of_isEmpty_eq_false
   -- To be proved from the concrete heap implementation
   simp [sizeOf]
   simp  [extract_min]
-  apply extractMinSize
+  apply extract_min_size
   apply notIsEmptyIsNotLeaf at hNE
   exact hNE
+
+
+def subTree (sub sup: BinaryTree α):= ∀ v, contains sub v → contains sup v
+
+-- def subTreeGE (sub sup: BinaryTree α) (hmin: is_min_heap sup f) ():= ∀ v y, contains sub v → contains sup v → contains sup y → f y ≤ f v
+
+
+-- lemma key_at_y_le_extracted_min_sub_tree [Nonempty α] [DecidableEq α] (y: α) (sub sup: BinaryTree α)
+--  (f: α → ENat) (hsup: extract_min sup f = y) (hsub: ¬ (contains sub y)) (hnesub: ¬ is_empty_tree sub) (hsubtree: subTree sub sup) (hmin: is_min_heap sup f):
+--  ∀ u, (BinaryTree.extract_min sub f).1 = some u → f y ≤ f u := by
+-- simp[BinaryTree.extract_min]
+-- have subp := sub
+-- cases sub.get_last.1
+-- . simp
+-- . simp
+--   cases sub.get_last.2
+--   . simp_all
+--     expose_names
+--     have: contains sub val := by sorry
+--     have: contains sup val := by
+--       simp [subTree] at hsubtree
+--       specialize hsubtree val this
+--       exact hsubtree
+--     grind
+--   . simp
+--     expose_names
+--     have: contains sub a_1 := by sorry
+--     have: contains sup a_1 := by
+--       simp [subTree] at hsubtree
+--       specialize hsubtree val this
+--       exact hsubtree
+
 
 -- minimimla heap-distance consistency lemma
 lemma key_at_y_le_extracted_min [Nonempty V] [DecidableEq V]
@@ -1166,20 +1203,20 @@ lemma key_at_y_le_extracted_min [Nonempty V] [DecidableEq V]
   -- smaller than the finalized key `y`.
   admit
 
-lemma decreasePriorityPreservesLeaf [DecidableEq α] (bt: BinaryTree α) (v: α) (f: α → ENat): bt = leaf → decreasePriority bt v f = leaf := by
-simp[decreasePriority]
+lemma decrease_priorityPreservesLeaf [DecidableEq α] (bt: BinaryTree α) (v: α) (f: α → ENat): bt = leaf → BinaryTree.decrease_priority bt v f = leaf := by
+simp[BinaryTree.decrease_priority]
 intro
 by_contra
 grind
 
-lemma decreasePriorityPreservesNode [DecidableEq α] (bt l r: BinaryTree α) (v v': α) (f: α → ENat): bt = node l v' r→  ∃ l' r' v'', decreasePriority bt v f = node l' v'' r' := by
+lemma decrease_priorityPreservesNode [DecidableEq α] (bt l r: BinaryTree α) (v v': α) (f: α → ENat): bt = node l v' r→  ∃ l' r' v'', BinaryTree.decrease_priority bt v f = node l' v'' r' := by
 intro hbt
-simp [decreasePriority]
-by_cases bt.containsB v
+simp [BinaryTree.decrease_priority]
+by_cases bt.containsb v
 . expose_names
   rw[h]
   simp_all
-  apply insertIsNode ((l.node v' r).remove v f) f v
+  apply insert_is_node ((l.node v' r).remove v f) f v
 . expose_names
   simp[h]
   use l
@@ -1195,13 +1232,13 @@ lemma decrease_priority_preserves_isEmpty [DecidableEq V] (q : BinaryHeap V) (v 
       simp [isEmpty] at h
       have: q.tree = leaf := by grind
       simp [decrease_priority, isEmpty]
-      apply decreasePriorityPreservesLeaf (q.tree) v d' at this
+      apply decrease_priorityPreservesLeaf (q.tree) v d' at this
       rw[this]
     . expose_names
       simp [isEmpty] at h
       have: ∃ l v' r, q.tree = node l v' r := by grind
       obtain ⟨l, v', r, h⟩ := this
-      obtain ⟨ l', v'', r', h'⟩ := decreasePriorityPreservesNode q.tree l r v v' d' h
+      obtain ⟨ l', v'', r', h'⟩ := decrease_priorityPreservesNode q.tree l r v v' d' h
       simp [decrease_priority]
       rw [h']
       simp[isEmpty]
